Test/civl/inductive-sequentialization/2PC.bpl
@@ -60,6 +60,8 @@ creates PARTICIPANT2;
 modifies RequestChannel, VoteChannel, DecisionChannel, votes, decisions;
 {
   var {:pool "INV4"} k: int;
+  var {:linear} pids': Set int;
+  var {:linear} participantPids: Set int;
 
   assert Init(pids->val, RequestChannel, VoteChannel, DecisionChannel, decisions);
 
@@ -73,7 +75,10 @@ modifies RequestChannel, VoteChannel, DecisionChannel, votes, decisions;
     (decisions[0] == COMMIT() ==> (forall i:int :: pid(i) ==> votes[i] == YES())) &&
     (forall i:int :: pidLe(i,k) ==> decisions[i] == decisions[0]);
   DecisionChannel := (lambda i:int :: (lambda d:decision :: if pidGt(i, k) && d == decisions[0] then 1 else 0));
-  call create_asyncs((lambda {:pool "PARTICIPANT2"} pa:PARTICIPANT2 :: pidGt(pa->pid->val, k)));
+
+  pids' := pids;
+  call participantPids := Set_Get(pids', (lambda i:int :: k < i && i <= n));
+  call {:linear participantPids} create_asyncs((lambda {:pool "PARTICIPANT2"} pa:PARTICIPANT2 :: pidGt(pa->pid->val, k)));
   call set_choice(PARTICIPANT2(One(k+1)));
 }
 
@@ -88,6 +93,9 @@ creates PARTICIPANT2;
 modifies RequestChannel, VoteChannel, DecisionChannel, votes, decisions;
 {
   var dec:decision;
+  var {:linear} pids': Set int;
+  var {:linear} participantPids: Set int;
+
   assert Init(pids->val, RequestChannel, VoteChannel, DecisionChannel, decisions);
 
   assume {:add_to_pool "INV4", 0} true;
@@ -96,7 +104,9 @@ modifies RequestChannel, VoteChannel, DecisionChannel, votes, decisions;
   assume dec == COMMIT() ==> (forall i:int :: pid(i) ==> votes[i] == YES());
   decisions[0] := dec;
   DecisionChannel := (lambda i:int :: (lambda d:decision :: if pid(i) && d == dec then 1 else 0));
-  call create_asyncs((lambda pa:PARTICIPANT2 :: pid(pa->pid->val)));
+  pids' := pids;
+  call participantPids := Set_Get(pids', (lambda i:int :: pid(i)));
+  call {:linear participantPids} create_asyncs((lambda pa:PARTICIPANT2 :: pid(pa->pid->val)));
 }
 
 ////////////////////////////////////////////////////////////////////////////////
@@ -106,13 +116,21 @@ refines MAIN4;
 creates COORDINATOR2, PARTICIPANT2;
 modifies RequestChannel, VoteChannel, votes;
 {
+  var {:linear} pids': Set int;
+  var {:linear} pid: One int;
+  var {:linear} participantPids: Set int;
+
   assert Init(pids->val, RequestChannel, VoteChannel, DecisionChannel, decisions);
+  
   havoc RequestChannel, VoteChannel, votes;
   assume VoteChannel[YES()] >= 0 && VoteChannel[NO()] >= 0;
   assume VoteChannel[YES()] + VoteChannel[NO()] <= n;
   assume VoteChannel[YES()] == n ==> (forall i:int :: pid(i) ==> votes[i] == YES());
-  call create_async(COORDINATOR2(One(0)));
-  call create_asyncs((lambda pa:PARTICIPANT2 :: pid(pa->pid->val)));
+  pids' := pids;
+  call pid := One_Get(pids', 0);
+  async call COORDINATOR2(pid);
+  call participantPids := Set_Get(pids', (lambda i:int :: pid(i)));
+  call {:linear participantPids} create_asyncs((lambda pa:PARTICIPANT2 :: pid(pa->pid->val)));
 }
 
 action {:layer 3}
@@ -120,6 +138,9 @@ INV2 ({:linear_in} pids: Set int)
 creates COORDINATOR2, PARTICIPANT1, PARTICIPANT2;
 modifies RequestChannel, VoteChannel, votes;
 {
+  var {:linear} pids': Set int;
+  var {:linear} pid: One int;
+  var {:linear} participantPids: Set int;
   var {:pool "INV2"} k: int;
 
   assert Init(pids->val, RequestChannel, VoteChannel, DecisionChannel, decisions);
@@ -133,9 +154,13 @@ modifies RequestChannel, VoteChannel, votes;
     VoteChannel[YES()] >= 0 && VoteChannel[NO()] >= 0 &&
     VoteChannel[YES()] + VoteChannel[NO()] <= k &&
     (VoteChannel[YES()] == k ==> (forall i:int :: pidLe(i,k) ==> votes[i] == YES()));
-  call create_async(COORDINATOR2(One(0)));
-  call create_asyncs((lambda pa:PARTICIPANT2 :: pidLe(pa->pid->val, k)));
-  call create_asyncs((lambda {:pool "PARTICIPANT1"} pa:PARTICIPANT1 :: pidGt(pa->pid->val, k)));
+  pids' := pids;
+  call pid := One_Get(pids', 0);
+  async call COORDINATOR2(pid);
+  call participantPids := Set_Get(pids', (lambda i:int :: 1 <= i && i <= k));
+  call {:linear participantPids} create_asyncs((lambda pa:PARTICIPANT2 :: pidLe(pa->pid->val, k)));
+  call participantPids := Set_Get(pids', (lambda i:int :: k < i && i <= n));
+  call {:linear participantPids} create_asyncs((lambda {:pool "PARTICIPANT1"} pa:PARTICIPANT1 :: pidGt(pa->pid->val, k)));
   call set_choice(PARTICIPANT1(One(k+1)));
 }
 
@@ -146,12 +171,19 @@ refines MAIN3 using INV2;
 creates COORDINATOR2, PARTICIPANT1;
 modifies RequestChannel;
 {
+  var {:linear} pids': Set int;
+  var {:linear} pid: One int;
+  var {:linear} participantPids: Set int;
+
   assert Init(pids->val, RequestChannel, VoteChannel, DecisionChannel, decisions);
 
   assume {:add_to_pool "INV2", 0} true;
   RequestChannel := (lambda i:int :: if pid(i) then 1 else 0);
-  call create_async(COORDINATOR2(One(0)));
-  call create_asyncs((lambda pa:PARTICIPANT1 :: pid(pa->pid->val)));
+  pids' := pids;
+  call pid := One_Get(pids', 0);
+  async call COORDINATOR2(pid);
+  call participantPids := Set_Get(pids', (lambda i:int :: pid(i)));
+  call {:linear participantPids} create_asyncs((lambda pa:PARTICIPANT1 :: pid(pa->pid->val)));
 }
 
 ////////////////////////////////////////////////////////////////////////////////
@@ -160,9 +192,17 @@ atomic action {:layer 2} MAIN1 ({:linear_in} pids: Set int)
 refines MAIN2;
 creates COORDINATOR1, PARTICIPANT1;
 {
+  var {:linear} pids': Set int;
+  var {:linear} pid: One int;
+  var {:linear} participantPids: Set int;
+  
   assert Init(pids->val, RequestChannel, VoteChannel, DecisionChannel, decisions);
-  call create_async(COORDINATOR1(One(0)));
-  call create_asyncs((lambda pa:PARTICIPANT1 :: pid(pa->pid->val)));
+
+  pids' := pids;
+  call pid := One_Get(pids', 0);
+  async call COORDINATOR1(pid);
+  call participantPids := Set_Get(pids', (lambda i:int :: pid(i)));
+  call {:linear participantPids} create_asyncs((lambda pa:PARTICIPANT1 :: pid(pa->pid->val)));
 }
 
 async atomic action {:layer 2,3} PARTICIPANT1 ({:linear_in} pid: One int)
@@ -181,7 +221,7 @@ modifies RequestChannel, VoteChannel, votes;
     VoteChannel[v] := VoteChannel[v] + 1;
   }
 
-  call create_async(PARTICIPANT2(pid));
+  async call PARTICIPANT2(pid);
 }
 
 async atomic action {:layer 2,5} PARTICIPANT2 ({:linear_in} pid: One int)
@@ -203,7 +243,7 @@ modifies RequestChannel;
 {
   assert pid->val == 0;
   RequestChannel := (lambda i:int :: if pid(i) then RequestChannel[i] + 1 else RequestChannel[i]);
-  call create_async(COORDINATOR2(One(0)));
+  async call COORDINATOR2(pid);
 }
 
 async atomic action {:layer 2,4} COORDINATOR2 ({:linear_in} pid: One int)
