Test/civl/paxos/PaxosSeq.bpl
@@ -11,7 +11,7 @@ creates A_StartRound;
     0 <= numRounds;
   joinedNodes := (lambda r: Round:: NoNodes());
   voteInfo := (lambda r: Round:: None());
-  call create_asyncs((lambda pa: A_StartRound :: AllPermissions(pa->r) == pa->r_lin && Round(pa->r) && pa->r <= numRounds));
+  call {:linear ps} create_asyncs((lambda pa: A_StartRound :: AllPermissions(pa->r) == pa->r_lin && Round(pa->r) && pa->r <= numRounds));
 }
 
 atomic action {:layer 3} A_Paxos'({:linear_in} ps: Set Permission)
@@ -26,13 +26,18 @@ action {:layer 2}
 INV({:linear_in} ps: Set Permission)
 creates A_StartRound, A_Propose, A_Conclude, A_Join, A_Vote;
 modifies joinedNodes, voteInfo, decision;
+requires Init(ps, decision);
 {
+  var {:linear} ps': Set Permission;
+  var {:linear} proposePermissions: Set Permission;
+  var {:linear} joinPermissions: Set Permission;
+  var {:linear} votePermissions: Set Permission;
+  var {:linear} concludePermission: One Permission;
   var {:pool "NumRounds"} numRounds: int;
   var {:pool "Round"} k: int;
   var {:pool "Node"} m: Node;
 
-  assert Init(ps, decision);
-
+  ps' := ps;
   havoc joinedNodes, voteInfo, decision;
 
   // This invariant is the "pending async skeleton" which states the possible
@@ -53,7 +58,7 @@ modifies joinedNodes, voteInfo, decision;
       assume
         (forall r: Round :: r < 1 || r > k ==> voteInfo[r] is None) &&
         (forall r: Round :: r < 1 || r > k ==> decision[r] is None);
-      call create_asyncs((lambda {:pool "A_StartRound"} pa: A_StartRound :: AllPermissions(pa->r) == pa->r_lin && k < pa->r && pa->r <= numRounds));
+      call {:linear ps'} create_asyncs((lambda {:pool "A_StartRound"} pa: A_StartRound :: AllPermissions(pa->r) == pa->r_lin && k < pa->r && pa->r <= numRounds));
       call set_choice(A_StartRound(k+1, AllPermissions(k+1)));
   } else if (*) {
       assume
@@ -63,11 +68,16 @@ modifies joinedNodes, voteInfo, decision;
         {:add_to_pool "Node", m}
         {:add_to_pool "A_Join", A_Join(k+1, numNodes, One(JoinPerm(k+1, numNodes)))}
         0 <= m && m <= numNodes;
-      call create_asyncs((lambda pa: A_StartRound :: AllPermissions(pa->r) == pa->r_lin && k+1 < pa->r && pa->r <= numRounds));
-      call create_async(A_Propose(k+1, ProposePermissions(k+1)));
-      call create_asyncs((lambda {:pool "A_Join"} pa: A_Join :: pa->r == k+1 && m < pa->n && pa->n <= numNodes && pa->p->val == JoinPerm(k+1, pa->n)));
-      if (m == numNodes) { call set_choice(A_Propose(k+1, ProposePermissions(k+1))); }
-      else { call set_choice(A_Join(k+1, m+1, One(JoinPerm(k+1, m+1)))); }
+      call proposePermissions := Set_Get(ps', ProposePermissions(k+1)->val);
+      async call A_Propose(k+1, proposePermissions);
+      call joinPermissions := Set_Get(ps', JoinPermissions(k+1)->val);
+      call {:linear joinPermissions} create_asyncs((lambda {:pool "A_Join"} pa: A_Join :: pa->r == k+1 && m < pa->n && pa->n <= numNodes && pa->p->val == JoinPerm(k+1, pa->n)));
+      call {:linear ps'} create_asyncs((lambda pa: A_StartRound :: AllPermissions(pa->r) == pa->r_lin && k+1 < pa->r && pa->r <= numRounds));
+      if (m == numNodes) {
+        call set_choice(A_Propose(k+1, ProposePermissions(k+1)));
+      } else {
+        call set_choice(A_Join(k+1, m+1, One(JoinPerm(k+1, m+1))));
+      }
   } else {
       assume
         voteInfo[k+1] is Some &&
@@ -79,11 +89,16 @@ modifies joinedNodes, voteInfo, decision;
         {:add_to_pool "A_StartRound", A_StartRound(numRounds, AllPermissions(numRounds))}
         0 <= m && m <= numNodes &&
         (forall n: Node :: n < 1 || n > m ==> !voteInfo[k+1]->t->ns[n]);
-      call create_asyncs((lambda {:pool "A_StartRound"} pa: A_StartRound :: AllPermissions(pa->r) == pa->r_lin && k+1 < pa->r && pa->r <= numRounds));
-      call create_async(A_Conclude(k+1, voteInfo[k+1]->t->value, One(ConcludePerm(k+1))));
-      call create_asyncs((lambda {:pool "A_Vote"} pa: A_Vote :: pa->r == k+1 && m < pa->n && pa->n <= numNodes && pa->v == voteInfo[k+1]->t->value && pa->p->val == VotePerm(k+1, pa->n)));
-      if (m == numNodes) { call set_choice(A_Conclude(k+1, voteInfo[k+1]->t->value, One(ConcludePerm(k+1)))); }
-      else { call set_choice(A_Vote(k+1, m+1, voteInfo[k+1]->t->value, One(VotePerm(k+1, m+1)))); }
+      call concludePermission := One_Get(ps', ConcludePerm(k+1));
+      async call A_Conclude(k+1, voteInfo[k+1]->t->value, concludePermission);
+      call votePermissions := Set_Get(ps', VotePermissions(k+1)->val);
+      call {:linear votePermissions} create_asyncs((lambda {:pool "A_Vote"} pa: A_Vote :: pa->r == k+1 && m < pa->n && pa->n <= numNodes && pa->v == voteInfo[k+1]->t->value && pa->p->val == VotePerm(k+1, pa->n)));
+      call {:linear ps'} create_asyncs((lambda {:pool "A_StartRound"} pa: A_StartRound :: AllPermissions(pa->r) == pa->r_lin && k+1 < pa->r && pa->r <= numRounds));
+      if (m == numNodes) {
+        call set_choice(A_Conclude(k+1, voteInfo[k+1]->t->value, One(ConcludePerm(k+1))));
+      } else {
+        call set_choice(A_Vote(k+1, m+1, voteInfo[k+1]->t->value, One(VotePerm(k+1, m+1))));
+      }
   }
 
   // If there was a decision for some value, then there must have been a
